Coq/src/SimRelCertStepCoh.v
@@ -1,0 +1,788 @@
+Require Import Omega.
+From hahn Require Import Hahn.
+From imm Require Import Events Execution
+     Traversal TraversalConfig SimTraversal SimTraversalProperties
+     Prog ProgToExecution ProgToExecutionProperties Receptiveness
+     imm_common imm_s imm_s_hb SimulationRel
+     CertExecution2 CertExecutionMain
+     SubExecution CombRelations AuxRel.
+Require Import AuxRel.
+Require Import AuxDef.
+Require Import EventStructure.
+Require Import Consistency.
+Require Import Execution.
+Require Import BasicStep.
+Require Import AddJF.
+Require Import AddEW.
+Require Import AddCO.
+Require Import Step.
+Require Import StepWf.
+Require Import LblStep.
+Require Import CertRf.
+Require Import CertGraph.
+Require Import EventToAction.
+Require Import ImmProperties.
+Require Import SimRelCont.
+Require Import SimRelEventToAction.
+Require Import SimRel.
+Require Import SimRelCert.
+Require Import SimRelCertBasicStep.
+Require Import SimRelAddJF.
+Require Import SimRelAddEW.
+Require Import SimRelAddCO.
+Require Import SimRelCertStep.
+Require Import ProgES.
+
+Set Implicit Arguments.
+Local Open Scope program_scope.
+
+Section SimRelCertStepCoh.
+
+  Variable prog : Prog.t.
+  Variable G : execution.
+  Variable sc : relation actid.
+  Variable TC : trav_config.
+  Variable TC' : trav_config.
+  Variable X : eventid -> Prop.
+
+  Notation "'SE' S" := S.(ES.acts_set) (at level 10).
+  Notation "'SEinit' S" := S.(ES.acts_init_set) (at level 10).
+  Notation "'SEninit' S" := S.(ES.acts_ninit_set) (at level 10).
+  Notation "'Stid' S" := (S.(ES.tid)) (at level 10).
+  Notation "'Slab' S" := S.(ES.lab) (at level 10).
+  Notation "'Sloc' S" := (Events.loc S.(ES.lab)) (at level 10).
+
+  Notation "'Ssb' S" := S.(ES.sb) (at level 10).
+  Notation "'Srmw' S" := S.(ES.rmw) (at level 10).
+  Notation "'Sew' S" := S.(ES.ew) (at level 10).
+  Notation "'Sjf' S" := S.(ES.jf) (at level 10).
+  Notation "'Srf' S" := S.(ES.rf) (at level 10).
+  Notation "'Sco' S" := S.(ES.co) (at level 10).
+  Notation "'Scf' S" := S.(ES.cf) (at level 10).
+
+  Notation "'Sjfe' S" := S.(ES.jfe) (at level 10).
+  Notation "'Srfe' S" := S.(ES.rfe) (at level 10).
+  Notation "'Scoe' S" := S.(ES.coe) (at level 10).
+  Notation "'Sjfi' S" := S.(ES.jfi) (at level 10).
+  Notation "'Srfi' S" := S.(ES.rfi) (at level 10).
+  Notation "'Scoi' S" := S.(ES.coi) (at level 10).
+
+  Notation "'Scc' S" := S.(cc) (at level 10).
+  Notation "'Ssw' S" := S.(sw) (at level 10).
+  Notation "'Shb' S" := S.(hb) (at level 10).
+  Notation "'Secf' S" := (S.(Consistency.ecf)) (at level 10).
+  Notation "'Seco' S" := (Consistency.eco S Weakestmo) (at level 10).
+
+  Notation "'SR' S" := (fun a => is_true (is_r S.(ES.lab) a)) (at level 10).
+  Notation "'SW' S" := (fun a => is_true (is_w S.(ES.lab) a)) (at level 10).
+  Notation "'SF' S" := (fun a => is_true (is_f S.(ES.lab) a)) (at level 10).
+
+  Notation "'SPln' S" := (fun a => is_true (is_only_pln S.(ES.lab) a)) (at level 10).
+  Notation "'SRlx' S" := (fun a => is_true (is_rlx S.(ES.lab) a)) (at level 10).
+  Notation "'SRel' S" := (fun a => is_true (is_rel S.(ES.lab) a)) (at level 10).
+  Notation "'SAcq' S" := (fun a => is_true (is_acq S.(ES.lab) a)) (at level 10).
+  Notation "'SAcqrel' S" := (fun a => is_true (is_acqrel S.(ES.lab) a)) (at level 10).
+  Notation "'SSc' S" := (fun a => is_true (is_sc S.(ES.lab) a)) (at level 10).
+
+  Notation "'K' S" := (S.(ES.cont_set)) (at level 10).
+
+  Notation "'Stid_' S" := (fun t x => Stid S x = t) (at level 1).
+  Notation "'SNTid_' S" := (fun t x => Stid S x <> t) (at level 1).
+
+  Notation "'GE'" := G.(acts_set).
+  Notation "'GEinit'" := (is_init ∩₁ GE).
+  Notation "'GEninit'" := ((set_compl is_init) ∩₁ GE).
+
+  Notation "'Glab'" := (Execution.lab G).
+  Notation "'Gloc'" := (Events.loc (lab G)).
+  Notation "'Gtid'" := (Events.tid).
+
+  Notation "'GTid' t" := (fun x => Gtid x = t) (at level 1).
+  Notation "'GNTid' t" := (fun x => Gtid x <> t) (at level 1).
+
+  Notation "'GR'" := (fun a => is_true (is_r Glab a)).
+  Notation "'GW'" := (fun a => is_true (is_w Glab a)).
+  Notation "'GF'" := (fun a => is_true (is_f Glab a)).
+
+  Notation "'GRel'" := (fun a => is_true (is_rel Glab a)).
+  Notation "'GAcq'" := (fun a => is_true (is_acq Glab a)).
+
+  Notation "'Gsb'" := (Execution.sb G).
+  Notation "'Grmw'" := (Execution.rmw G).
+  Notation "'Grf'" := (Execution.rf G).
+  Notation "'Gco'" := (Execution.co G).
+
+  Notation "'Grs'" := (imm_s_hb.rs G).
+  Notation "'Grelease'" := (imm_s_hb.release G).
+  Notation "'Gsw'" := (imm_s_hb.sw G).
+  Notation "'Ghb'" := (imm_s_hb.hb G).
+
+  Notation "'Gfurr'" := (furr G sc).
+  Notation "'Gvf' t" := (vf G sc TC' t) (at level 10, only parsing).
+
+  Notation "'Geco'" := (Execution_eco.eco G).
+
+  Notation "'C'"  := (covered TC).
+  Notation "'I'"  := (issued TC).
+  Notation "'C''"  := (covered TC').
+  Notation "'I''"  := (issued TC').
+
+  Notation "'thread_syntax' t"  := 
+    (Language.syntax (thread_lts t)) (at level 10, only parsing).  
+
+  Notation "'thread_st' t" := 
+    (Language.state (thread_lts t)) (at level 10, only parsing).
+
+  Notation "'thread_init_st' t" := 
+    (Language.init (thread_lts t)) (at level 10, only parsing).
+
+  Notation "'thread_cont_st' t" :=
+    (fun st => existT _ (thread_lts t) st) (at level 10, only parsing).
+
+  Notation "'cont_lang'" :=
+    (fun S k => thread_lts (ES.cont_thread S k)) (at level 10, only parsing).
+
+  Notation "'kE' S" := (fun k => ES.cont_sb_dom S k) (at level 1, only parsing).
+  Notation "'ktid' S" := (fun k => ES.cont_thread S k) (at level 1, only parsing).
+
+  Notation "'certX' S" := (fun k => (X ∩₁ SNTid_ S (ktid S k)) ∪₁ (kE S k)) (at level 1, only parsing).
+
+  Lemma simrel_cert_step_hb_delta_dom k k' e e' S S'
+        (st st' st'': (thread_st (ktid S k)))
+        (SRCC : simrel_cert prog S G sc TC TC' X k st st'') 
+        (CertSTEP : cert_step G sc TC TC' X k k' st st' e e' S S')
+        (CST_REACHABLE : (lbl_step (ktid S k))＊ st' st'') : 
+    dom_rel (hb_delta S S' k e e') ⊆₁ certX S k ∪₁ eq e.
+  Proof. 
+    cdes CertSTEP; cdes BSTEP_.
+    assert (basic_step e e' S S') as BSTEP.
+    { econstructor; eauto. }
+    assert (step_ e e' S S') as WMO_STEP_.
+    { eapply simrel_cert_step_step_; eauto. }
+    assert (ES.Wf S) as WFS.
+    { apply SRCC. }
+    unfold hb_delta. relsf. split. 
+    { rewrite <- seqA, dom_seq.
+      eapply simrel_cert_basic_step_hb_sb_delta_dom; eauto. }
+    unfold_cert_step_ CertSTEP_.
+    all : rewrite <- seqA, dom_seq.
+    2,4 : left; eapply sim_add_jf_hb_sw_delta_dom; eauto. 
+    all : unfold sw_delta.
+    all : rewrite JF'; relsf; rewrite !seqA; splits.
+    2,4 : step_solver.
+    all : do 3 rewrite <- seqA; rewrite dom_seq, !seqA.
+    all : left; eapply simrel_cert_basic_step_hb_rel_jf_sb_delta_dom; eauto.
+  Qed.
+
+  Lemma simrel_cert_step_hb_cf_irr k k' e e' S S'
+        (st st' st'': (thread_st (ktid S k)))
+        (SRCC : simrel_cert prog S G sc TC TC' X k st st'')
+        (CertSTEP : cert_step G sc TC TC' X k k' st st' e e' S S')
+        (CST_REACHABLE : (lbl_step (ktid S k))＊ st' st'') : 
+    irreflexive (Shb S' ⨾ Scf S').
+  Proof.
+    cdes CertSTEP; cdes BSTEP_.
+    assert (basic_step e e' S S') as BSTEP.
+    { econstructor; eauto. }
+    assert (step_ e e' S S') as WMO_STEP_.
+    { eapply simrel_cert_step_step_; eauto. }
+    assert (ES.Wf S) as WFS.
+    { apply SRCC. }
+    erewrite step_hb; eauto.
+    erewrite basic_step_cf; eauto.
+    relsf. rewrite !irreflexive_union. splits.
+
+    { eapply ecf_irr_hb_cf_irr. apply SRCC. }
+
+    { step_solver. } 
+
+    { autounfold with ESStepDb.
+      rewrite !csE, !transp_cross.
+      relsf. rewrite !irreflexive_union. splits.
+      2,4 : by step_solver.
+      { intros x [y [HB [KCF EQe]]].
+        subst x. apply hbE, seq_eqv_lr in HB; auto. desf.
+        eapply basic_step_acts_set_ne; eauto. }
+      unfold eq_opt. destruct e' as [e'|]; [|basic_solver].
+      intros x [y [HB [KCF EQOPTe]]].
+      subst x. apply hbE, seq_eqv_lr in HB; auto. desf.
+      eapply basic_step_acts_set_ne'; eauto. }
+
+    unfold cf_delta.
+    rewrite !csE, !transp_cross. relsf.
+    arewrite_false (hb_delta S S' k e e' ⨾ ES.cont_cf_dom S k × eq e).
+    { step_solver. }
+    arewrite_false (hb_delta S S' k e e' ⨾ ES.cont_cf_dom S k × eq_opt e'). 
+    { step_solver. }
+    relsf.
+
+    erewrite dom_rel_helper with (r := hb_delta S S' k e e').
+    2 : { eapply simrel_cert_step_hb_delta_dom; eauto. }
+    rewrite id_union. 
+    relsf. rewrite !irreflexive_union. splits.
+    all : try by step_solver.
+    all : unfolder; ins; desc. 
+    all : eapply certX_ncf_cont; eauto.
+    all : basic_solver.
+  Qed.
+
+  Lemma simrel_cert_step_thb_cf_hb_irr k k' e e' S S'
+        (st st' st'': (thread_st (ktid S k)))
+        (SRCC : simrel_cert prog S G sc TC TC' X k st st'')
+        (CertSTEP : cert_step G sc TC TC' X k k' st st' e e' S S')
+        (CST_REACHABLE : (lbl_step (ktid S k))＊ st' st'') : 
+    irreflexive ((Shb S')⁻¹ ⨾ (Scf S') ⨾ (Shb S')).
+  Proof.
+    cdes CertSTEP; cdes BSTEP_.
+    assert (basic_step e e' S S') as BSTEP.
+    { econstructor; eauto. }
+    assert (step_ e e' S S') as WMO_STEP_.
+    { eapply simrel_cert_step_step_; eauto. }
+    assert (ES.Wf S) as WFS.
+    { apply SRCC. }
+    erewrite step_hb; eauto.
+    erewrite basic_step_cf; eauto.
+    unfold cf_delta.
+    erewrite dom_rel_helper with (r := hb_delta S S' k e e').
+    2 : { eapply simrel_cert_step_hb_delta_dom; eauto. }
+    rewrite !transp_union.
+    relsf. rewrite !irreflexive_union. splits.
+
+    { eapply ecf_irr_thb_cf_hb_irr. apply SRCC. }
+
+    1-8 : step_solver.
+
+    all : rewrite !id_union with (s := certX S k) (s' := eq e).
+    all : rewrite !transp_seq, !transp_union, !transp_eqv_rel. 
+    all : relsf; rewrite !seqA.
+
+    { arewrite_false (Scf S ⨾ ⦗eq e⦘).
+      { step_solver. }
+      arewrite_false (⦗eq e⦘ ⨾ Scf S).
+      { step_solver. }
+      relsf. 
+      unfolder. ins. desc. subst.
+      eapply cert_ex_ncf; eauto. 
+      unfolder. eauto 20. }
+
+    { erewrite cert_ex_inE at 1 2; eauto.
+      arewrite_false 
+        (⦗SE S⦘ ⨾ (ES.cont_cf_dom S k × eq e) ^⋈ ⨾ ⦗SE S⦘).
+      { step_solver. }
+      arewrite_false 
+      (⦗eq e⦘ ⨾ (ES.cont_cf_dom S k × eq e) ^⋈ ⨾ ⦗eq e⦘).
+      { step_solver. }
+      relsf.
+
+      rewrite !csE. relsf.
+      arewrite_false (eq e × ES.cont_cf_dom S k ⨾ ⦗eq e⦘).
+      { step_solver. }
+      arewrite_false (⦗eq e⦘ ⨾ ES.cont_cf_dom S k × eq e).
+      { step_solver. }
+      relsf. rewrite !irreflexive_union. splits.
+      all : unfolder; ins; desc; subst.
+      all : eapply certX_ncf_cont; eauto.
+      all : basic_solver. }
+
+    erewrite cert_ex_inE; eauto.
+    arewrite_false 
+      (⦗SE S⦘ ⨾ (ES.cont_cf_dom S k × eq_opt e') ^⋈ ⨾ ⦗SE S⦘).
+    { step_solver. }
+    arewrite_false 
+    (⦗SE S⦘ ⨾ (ES.cont_cf_dom S k × eq_opt e') ^⋈ ⨾ ⦗eq e⦘).
+    { step_solver. }
+    arewrite_false 
+    (⦗eq e⦘ ⨾ (ES.cont_cf_dom S k × eq_opt e') ^⋈ ⨾ ⦗SE S⦘).
+    { step_solver. }
+    arewrite_false 
+    (⦗eq e⦘ ⨾ (ES.cont_cf_dom S k × eq_opt e') ^⋈ ⨾ ⦗eq e⦘).
+    { step_solver. }
+    basic_solver.
+  Qed.
+
+  Lemma simrel_cert_step_jf_necf k k' e e' S S'
+        (st st' st'': (thread_st (ktid S k)))
+        (SRCC : simrel_cert prog S G sc TC TC' X k st st'')
+        (CertSTEP : cert_step G sc TC TC' X k k' st st' e e' S S')
+        (CST_REACHABLE : (lbl_step (ktid S k))＊ st' st'') : 
+    Sjf S' ∩ Secf S' ≡ ∅₂. 
+  Proof. 
+    cdes CertSTEP; cdes BSTEP_.
+    assert (basic_step e e' S S') as BSTEP.
+    { econstructor; eauto. }
+    assert (step_ e e' S S') as WMO_STEP_.
+    { eapply simrel_cert_step_step_; eauto. }
+    assert (ES.Wf S) as WFS.
+    { apply SRCC. }
+    unfold_cert_step_ CertSTEP_.
+    1,3 : 
+      eapply step_same_jf_jf_necf; 
+      eauto; try apply SRCC;
+        eapply basic_step_nupd_rmw;
+        subst; eauto.
+    { eapply sim_add_jf_jf_necf; eauto.
+      subst. basic_solver. }
+    eapply sim_add_jf_jf_necf; eauto.
+    cdes AEW. type_solver.
+  Qed.
+
+  Lemma simrel_cert_step_jfe_vis k k' e e' S S'
+        (st st' st'': (thread_st (ktid S k)))
+        (SRCC : simrel_cert prog S G sc TC TC' X k st st'')
+        (CertSTEP : cert_step G sc TC TC' X k k' st st' e e' S S')
+        (CST_REACHABLE : (lbl_step (ktid S k))＊ st' st'') : 
+    dom_rel (Sjfe S') ⊆₁ (vis S'). 
+  Proof. 
+    cdes CertSTEP; cdes BSTEP_.
+    assert (basic_step e e' S S') as BSTEP.
+    { econstructor; eauto. }
+    assert (step_ e e' S S') as WMO_STEP_.
+    { eapply simrel_cert_step_step_; eauto. }
+    assert (ES.Wf S) as WFS by apply SRCC.
+    etransitivity. 
+    2 : eapply step_vis_mon; eauto.
+    unfold_cert_step_ CertSTEP_.
+    all : try (by eapply sim_add_jf_jfe_vis; eauto).
+    all : rewrite step_same_jf_jfe; eauto; apply SRCC.
+  Qed.
+
+  Lemma simrel_cert_step_fr_simpl_coh k k' e e' S S'
+        (st st' st'': (thread_st (ktid S k)))
+        (SRCC : simrel_cert prog S G sc TC TC' X k st st'')
+        (CertSTEP : cert_step G sc TC TC' X k k' st st' e e' S S')
+        (CST_REACHABLE : (lbl_step (ktid S k))＊ st' st'') : 
+    irreflexive (Sco S' ⨾ (Sjf S')^? ⨾ Shb S' ⨾ (Sjf S')⁻¹).
+  Proof. 
+    cdes CertSTEP; cdes BSTEP_.
+    assert (basic_step e e' S S') as BSTEP.
+    { econstructor; eauto. }
+    assert (step_ e e' S S') as WMO_STEP_.
+    { eapply simrel_cert_step_step_; eauto. }
+    assert (ES.Wf S) as WF by apply SRCC.
+    assert (ES.Wf S') as WFS.
+    { eapply step_wf; eauto. }
+    assert (simrel_e2a S' G sc) as SRE2A.
+    { eapply simrel_cert_step_e2a; eauto. }
+    assert (Wf G) as WFG. 
+    { apply SRCC. }
+    assert (coherence G) as GCOH.
+    { eapply gcons. apply SRCC. }
+
+    assert (irreflexive (Sco S ⨾ (Sjf S)^? ⨾ Shb S ⨾ (Sjf S)⁻¹))
+      as OLDCOH.
+    { apply irreflexive_seqC. rewrite !seqA. 
+      apply irreflexive_seqC. rewrite !seqA. 
+      rewrite WF.(ES.jf_in_rf).
+      arewrite ((Srf S)⁻¹ ⨾ Sco S ⊆ ES.fr S).
+      arewrite (ES.fr S ⨾ (Srf S)^? ⊆ (Seco S)^?).
+      2: by apply SRCC.
+      rewrite fr_in_eco.
+      arewrite (Srf S ⊆ Seco S).
+      generalize (eco_trans S Weakestmo).
+      basic_solver. }
+
+    assert 
+    (irreflexive (Sco S' ⨾ (Sjf S')^? ⨾ Shb S' ⨾ (Sjf S)⁻¹)) 
+      as IrrH.
+    { arewrite (Shb S' ⨾ (Sjf S)⁻¹ ≡ Shb S ⨾ (Sjf S)⁻¹).
+      { rewrite ES.jfE; auto.
+        rewrite !transp_seq, !transp_eqv_rel.
+        rewrite <- seq_eqvK at 1. 
+        rewrite !seqA, <- seqA.
+        arewrite (Shb S' ⨾ ⦗SE S⦘ ≡ Shb S); auto.
+        unfold_cert_step_ CertSTEP_.
+        1,3: 
+          eapply step_same_jf_hbE; eauto;
+          rewrite RMW'; subst; 
+            autounfold with ESStepDb;
+            basic_solver.
+        all: eapply add_jf_hbE; eauto. 
+        1,3 : eapply weaken_sim_add_jf; eauto.
+        { subst; autounfold with ESStepDb; basic_solver. }
+        cdes ACO. type_solver. }
+      arewrite ((Sjf S')^? ⨾ Shb S ≡ (Sjf S)^? ⨾ Shb S).
+      { rewrite !crE. relsf.
+        apply union_more; auto.
+        rewrite hbE; auto.
+        rewrite <- seq_eqvK at 1.
+        rewrite !seqA. 
+        arewrite (Sjf S' ⨾ ⦗SE S⦘ ≡ Sjf S); auto.
+        unfold_cert_step_ CertSTEP_.
+        1,3: rewrite JF', ES.jfE; basic_solver.
+        all : 
+          eapply add_jf_jfE; eauto;
+          eapply weaken_sim_add_jf; eauto. }
+      unfold_cert_step_ CertSTEP_.
+      all: try cdes ACO; rewrite CO'.
+      1,2: done.
+      all: unfold co_delta.
+      all: rewrite add_co_ws_complE; auto.
+      all: rewrite sim_wsE.
+      all: relsf.
+      all: rewrite !irreflexive_union; splits. 
+      2,3,5,6 : step_solver.
+      all: done. }
+
+    assert (e2a S' □ Ssb S' ⊆ Gsb) as SBN.
+    { eapply e2a_sb; eauto; try apply SRCC.
+      eapply e2a_GE; eauto. }
+    
+    assert (e2a S' □ Shb S' ⊆ Ghb) as HBN.
+    { admit. }
+
+    (* assert (e2a S' □ Sco S' ⨾ Sjf S' ⨾ Shb S' ⨾ ⦗eq e⦘ ⊆ *)
+    (*             Gco ⨾ vf G sc TC' (ES.cont_thread S k)) as COVF_H. *)
+    (* { admit. } *)
+    (* { arewrite (Sjf S' ⨾ Shb S' ⨾ ⦗eq e⦘ ⊆ Sjf S ⨾ Shb S' ⨾ ⦗eq e⦘). *)
+    (*   { admit. } *)
+    (*   rewrite !collect_rel_seqi. *)
+    (*   rewrite e2a_co; eauto. *)
+    (*   rewrite HBN. *)
+    (*   arewrite_id (e2a S' □ ⦗eq e⦘). *)
+    (*   { basic_solver. } *)
+    (*   rewrite seq_id_r. *)
+    (*   hahn_frame. *)
+    (*   arewrite (e2a S' □ Sjf S ⊆ e2a S □ Sjf S). *)
+    (*   { (* TODO: generalize to a lemma *) *)
+    (*     rewrite WF.(ES.jfE) at 1. *)
+    (*     unfolder. ins. desf. do 2 eexists. *)
+    (*     splits; eauto. *)
+    (*     all: symmetry; eapply basic_step_e2a_eq_dom; eauto. } *)
+    (*   arewrite (e2a S □ Sjf S ⊆ vf G sc TC' (ES.cont_thread S k)). *)
+    (*   { (* TODO: It should follow from the simulation invariant. *) *)
+    (*     admit. } *)
+    (*   unfold vf at 1. rewrite !seqA. *)
+    (*   arewrite (Ghb^? ⨾ ⦗GE⦘ ⨾ Ghb ⊆ Ghb^? ⨾ ⦗GE⦘). *)
+    (*   2: done. *)
+    (*   rewrite (dom_r WFG.(wf_hbE)) at 2. *)
+    (*   generalize (@imm_s_hb.hb_trans G). *)
+    (*   basic_solver 10. } *)
+
+    (* assert  *)
+    (*   (e2a S' □ Sco S' ⨾ (Sjf S')^? ⨾ Shb S' ⨾ ⦗ eq e ⦘ ⊆  *)
+    (*        Gco ⨾ Gvf (ktid S k)) *)
+    (*   as COVF. *)
+    (* { rewrite crE. rewrite !seq_union_l, !seq_union_r, seq_id_l. *)
+    (*   rewrite collect_rel_union. *)
+    (*   unionL; auto. *)
+    (*   rewrite !collect_rel_seqi. *)
+    (*   rewrite e2a_co; eauto. *)
+    (*   sin_rewrite HBN. *)
+    (*   arewrite_id (e2a S' □ ⦗eq e⦘). *)
+    (*   { basic_solver. } *)
+    (*   rewrite seq_id_r. *)
+    (*   rewrite (dom_r WFG.(wf_coD)) at 1. *)
+    (*   rewrite (dom_r WFG.(wf_hbE)) at 1. *)
+    (*   rewrite !seqA. *)
+    (*   do 2 hahn_frame. *)
+    (*   basic_solver 40. } *)
+
+    (* TODO: introduce a lemma *)
+    assert (Sjf S' ⨾ ⦗SE S⦘ ≡ Sjf S) as JFE.
+    { red in WMO_STEP_. desf; cdes WMO_STEP_.
+      1,3: rewrite JF', ES.jfE; auto; basic_solver.
+      all: erewrite add_jf_jfE; eauto. }
+
+    assert (irreflexive
+              ((e2a S' □ Sco S' ⨾ (Sjf S')^? ⨾ Shb S' ⨾ ⦗eq e⦘)
+                 ⨾ (cert_rf G sc TC' (ES.cont_thread S k))⁻¹)) as IRR.
+    { arewrite (Shb S' ⊆ ⦗X ∩₁ e2a S ⋄₁ covered TC⦘ ⨾ Shb S' ∪ Ssb S').
+      { (* TODO: hb_in_ex_cov_hb_sb requires too much. *)
+        admit. }
+      rewrite !seq_union_l, !seq_union_r, !seqA.
+      arewrite ((Sjf S')^? ⨾ ⦗X ∩₁ e2a S ⋄₁ C⦘ ⊆
+                        (Sjf S' ⨾ ⦗X ∩₁ e2a S ⋄₁ C⦘)^? ⨾ ⦗X ∩₁ e2a S ⋄₁ C⦘)
+        by basic_solver 10.
+      arewrite ((Sjf S')^? ⨾ Ssb S' ⨾ ⦗eq e⦘ ⊆ (Sjf S)^? ⨾ Ssb S' ⨾ ⦗eq e⦘).
+      { rewrite !crE. relsf.
+        apply union_mori; [done|].
+        erewrite basic_step_sbe; eauto.
+        erewrite dom_rel_helper 
+          with (r := ES.cont_sb_dom S k × eq e) (d := SE S) at 1.
+        { rewrite <- seqA. by rewrite JFE. }
+        rewrite dom_cross.
+        { eapply kE_inE; eauto. }
+        intros [HA HB]. by eapply HA. }
+      arewrite ((Sjf S)^? ⨾ Ssb S' ⨾ ⦗eq e⦘ ⊆
+                       (Sjf S ⨾ ⦗kE S k⦘)^? ⨾ Ssb S' ⨾ ⦗eq e⦘).
+      { erewrite basic_step_sbe; eauto. basic_solver 10. }
+
+      rewrite !collect_rel_union.
+      rewrite !collect_rel_seqi.
+      rewrite !collect_rel_cr.
+      arewrite (Sjf S' ⨾ ⦗X ∩₁ e2a S ⋄₁ C⦘ ⊆ 
+                    Sjf S ⨾ ⦗X ∩₁ e2a S ⋄₁ C⦘).
+      { rewrite <- seq_eqvK at 1.
+        arewrite (X ∩₁ e2a S ⋄₁ C ⊆₁ SE S) at 1.
+        { apply set_subset_inter_l. left.
+          rewrite Execution.ex_inE; eauto.
+          apply SRCC. }
+          by rewrite <- seqA, JFE. }
+      arewrite (e2a S' □ Sjf S ⨾ ⦗X ∩₁ e2a S ⋄₁ C⦘ ⊆
+                    e2a S  □ Sjf S  ⨾ ⦗X ∩₁ e2a S ⋄₁ C⦘).
+      { rewrite ES.jfE; auto.
+        rewrite !seqA, seq_eqvC.
+        arewrite (⦗SE S⦘ ⨾ Sjf S ⨾ ⦗X ∩₁ e2a S ⋄₁ C⦘ ⨾ ⦗SE S⦘ ≡ 
+                         restr_rel (SE S) (Sjf S ⨾ ⦗X ∩₁ e2a S ⋄₁ C⦘)).
+        { basic_solver. }
+        apply collect_rel_restr_eq_dom.
+        red. ins. symmetry. 
+        eapply basic_step_e2a_eq_dom; eauto. }
+      arewrite (e2a S □ Sjf S ⨾ ⦗X ∩₁ e2a S ⋄₁ C⦘ ⊆ Grf ⨾ ⦗C⦘).
+      { rewrite <- seq_eqvK, <- seqA. rewrite collect_rel_seqi.
+        arewrite (e2a S □ ⦗X ∩₁ e2a S ⋄₁ C⦘ ⊆ ⦗C⦘) by basic_solver. 
+          by rewrite jf_cov_in_rf; [|apply SRCC]. }
+      rewrite e2a_co; eauto.
+      rewrite HBN, SBN.
+      arewrite_id (e2a S' □ ⦗X ∩₁ e2a S ⋄₁ C⦘).
+      { basic_solver. }
+      rewrite seq_id_l.
+      rewrite !seq_union_l.
+      apply irreflexive_union; split.
+      { arewrite_id (e2a S' □ ⦗eq e⦘).
+        { basic_solver. }
+        rewrite seq_id_l.
+        rewrite (dom_r WFG.(wf_coD)), !seqA.
+        unfold cert_rf.
+        arewrite (⦗GW⦘ ⨾ (Grf ⨾ ⦗C⦘)^? ⨾ Ghb ⊆ vf G sc TC' (ES.cont_thread S k)).
+        2: basic_solver 20.
+        unfold vf.
+        unionR left.
+        arewrite (C ⊆₁ C').
+        { eapply sim_trav_step_covered_le.
+          eexists. apply SRCC. }
+        rewrite wf_hbE at 1; auto.
+        basic_solver 40. }
+      arewrite (e2a S' □ Sjf S ⨾ ⦗ES.cont_sb_dom S k⦘ ⊆
+                    e2a S  □ Sjf S ⨾ ⦗ES.cont_sb_dom S k⦘).
+      { rewrite ES.jfE at 1; auto.
+        unfolder. ins. desf. do 2 eexists. splits; eauto.
+        all: symmetry; eapply basic_step_e2a_eq_dom; eauto. }
+      rewrite jf_in_cert_rf; eauto.
+      rewrite (dom_r WFG.(wf_coD)), !seqA.
+      arewrite (⦗GW⦘ ⨾ (cert_rf G sc TC' (ES.cont_thread S k))^? ⨾ Gsb ⊆
+                     vf G sc TC' (ES.cont_thread S k)).
+      2: unfold cert_rf; basic_solver 10.
+      rewrite cert_rf_in_vf.
+      rewrite crE.
+      rewrite !seq_union_l, !seq_union_r, seq_id_l.
+      unionL.
+      { unfold vf.
+        unionR left.
+        rewrite imm_s_hb.sb_in_hb.
+        rewrite imm_s_hb.wf_hbE at 1; auto.
+        basic_solver 20. }
+      unfold vf at 1.
+      rewrite !seq_union_l, !seq_union_r, !seqA.
+      arewrite (Gsb^? ⨾ Gsb ⊆ Gsb^?).
+      { generalize (@Execution.sb_trans G). basic_solver. }
+      arewrite (Ghb^? ⨾ ⦗GE⦘ ⨾ Gsb ⊆ Ghb^? ⨾ ⦗GE⦘).
+      { rewrite Execution.wf_sbE. rewrite imm_s_hb.sb_in_hb.
+        generalize (@imm_s_hb.hb_trans G).
+        basic_solver. }
+      arewrite (⦗GW⦘ ⨾ Grf ⊆ Grf).
+      arewrite (⦗GW⦘ ⨾ ⦗GW⦘ ⊆ ⦗GW⦘).
+      done. }
+
+    unfold_cert_step_ CertSTEP_.
+    1,3: by rewrite JF' at 2. 
+    all: cdes AJF; rewrite JF' at 2.
+    all: rewrite transp_union; relsf.
+    all: rewrite !irreflexive_union; splits. 
+    1,3: done.
+
+    all: arewrite ((jf_delta w e)⁻¹ ≡
+                                 ⦗ eq e ⦘ ⨾ (jf_delta w e)⁻¹)
+      by (unfold jf_delta; basic_solver).
+    all: do 3 rewrite <- seqA.
+    all: rewrite seqA with (r1 := Sco S' ⨾ (Sjf S')^?).
+    all: rewrite seqA with (r1 := Sco S').
+    all: eapply collect_rel_irr with (f := e2a S').
+    all: rewrite collect_rel_seqi.
+    all: arewrite (e2a S' □ (jf_delta w e)⁻¹ ⊆ 
+                       (cert_rf G sc TC' (ktid S k))⁻¹)
+      by (unfold jf_delta; basic_solver).
+    
+    (* The old proof which requires DR restrictions *)
+    
+    (* (* TODO: introduce a corresponding lemma. *) *)
+    (* arewrite (Sjf S' ⊆ SimRelJF.sim_jf G sc TC' S' (certX S' k')). *)
+    (* { (* eapply jf_in_sim_jf. *) *)
+    (*   (* apply inclusion_minus_l. *) *)
+    (*   (* unionR right. *) *)
+    (*   (* Sew ;; sim_jf ⊆ sim_jf *) *)
+    (*   admit. } *)
+
+    (* arewrite (SimRelJF.sim_jf G sc TC' S' (certX S' k') ⊆ *)
+    (*           SimRelJF.sim_vf G sc TC' S' (certX S' k')) at 1. *)
+    (* arewrite (Sco S' ⨾ (SimRelJF.sim_vf G sc TC' S' (certX S' k'))^? ⨾ Shb S' ⊆ *)
+    (*           Sco S' ⨾ SimRelJF.sim_vf G sc TC' S' (certX S' k')). *)
+    (* 2: { unfold SimRelJF.sim_jf. basic_solver 10. } *)
+    (* rewrite crE. rewrite !seq_union_l, !seq_union_r, seq_id_l. *)
+    (* unionL. *)
+    (* 2: { arewrite (SimRelJF.sim_vf G sc TC' S' (certX S' k') ⨾ Shb S' ⊆ *)
+    (*                SimRelJF.sim_vf G sc TC' S' (certX S' k')). *)
+    (*      2: done. *)
+    (*      unfold SimRelJF.sim_vf. *)
+    (*      rewrite !seqA. *)
+    (*      arewrite ((Shb S')^? ⨾ Shb S' ⊆ (Shb S')^?). *)
+    (*      2: done. *)
+    (*      generalize (@hb_trans S'). basic_solver 20. } *)
+    (* unfold SimRelJF.sim_vf. *)
+    (* arewrite (Sco S' ⊆ Sco S' ⨾ Sew S'). *)
+    (* 2: basic_solver 20. *)
+    (* rewrite <- ES.ew_refl; auto. *)
+    (* rewrite (dom_r WFS.(ES.coD)) at 1. *)
+    (* rewrite (dom_r WFS.(ES.coE)) at 1. *)
+    (* basic_solver. *)
+  Admitted.
+
+  Lemma simrel_cert_step_fr_coh k k' e e' S S'
+        (st st' st'': (thread_st (ktid S k)))
+        (SRCC : simrel_cert prog S G sc TC TC' X k st st'')
+        (CertSTEP : cert_step G sc TC TC' X k k' st st' e e' S S')
+        (CST_REACHABLE : (lbl_step (ktid S k))＊ st' st'') : 
+    irreflexive (Shb S' ⨾ ES.fr S' ⨾ (Srf S')^?).
+  Proof. 
+    cdes CertSTEP; cdes BSTEP_.
+    assert (basic_step e e' S S') as BSTEP.
+    { econstructor; eauto. }
+    assert (step_ e e' S S') as WMO_STEP_.
+    { eapply simrel_cert_step_step_; eauto. }
+    assert (ES.Wf S) as WF by apply SRCC.
+    assert (ES.Wf S') as WFS.
+    { eapply step_wf; eauto. }
+
+    unfold ES.fr.
+    rewrite <- !seqA. apply irreflexive_seqC.
+    rewrite <- !seqA. apply irreflexive_seqC.
+    
+    arewrite (Srf S' ⊆ Sew S' ;; Sjf S').
+    arewrite ((Sew S' ⨾ Sjf S')^? ⊆ (Sew S')^? ⨾ (Sjf S')^?)
+      by basic_solver 10.
+    rewrite transp_seq.
+    arewrite (Sco S' ⨾ (Sew S')^? ⊆ Sco S').
+    { generalize WFS.(ES.co_ew_in_co). basic_solver. }
+    rewrite <- !seqA.
+    rewrite irreflexive_seqC.
+    rewrite !seqA.
+    arewrite ((Sew S')⁻¹ ⊆ Sew S').
+    { rewrite transp_sym_equiv; [done|]. apply WFS. }
+    sin_rewrite WFS.(ES.ew_co_in_co).
+    eapply simrel_cert_step_fr_simpl_coh; eauto.
+  Qed.
+
+  Lemma simrel_cert_step_coh k k' e e' S S'
+        (st st' st'': (thread_st (ktid S k)))
+        (SRCC : simrel_cert prog S G sc TC TC' X k st st'')
+        (CertSTEP : cert_step G sc TC TC' X k k' st st' e e' S S')
+        (CST_REACHABLE : (lbl_step (ktid S k))＊ st' st'') : 
+    irreflexive (Shb S' ⨾ (Seco S')^?).
+  Proof. 
+    cdes CertSTEP; cdes BSTEP_.
+    assert (basic_step e e' S S') as BSTEP.
+    { econstructor; eauto. }
+    assert (step_ e e' S S') as WMO_STEP_.
+    { eapply simrel_cert_step_step_; eauto. }
+    assert (ES.Wf S) as WF by apply SRCC.
+    assert (ES.Wf S') as WFS.
+    { eapply step_wf; eauto. }
+    assert (simrel_e2a S' G sc) as SRE2A.
+    { eapply simrel_cert_step_e2a; eauto. }
+    assert (Wf G) as WFG. 
+    { apply SRCC. }
+    assert (coherence G) as GCOH.
+    { eapply gcons. apply SRCC. }
+    
+    rewrite crE. rewrite eco_alt; auto.
+    rewrite crE at 1.
+    rewrite !seq_union_r, !seq_id_r.
+    rewrite <- !unionA.
+    apply irreflexive_union. splits.
+    2: by eapply simrel_cert_step_fr_coh; eauto.
+    eapply collect_rel_irr with (f := e2a S').
+    rewrite !collect_rel_union.
+    rewrite !collect_rel_seqi.
+    erewrite e2a_hb; eauto; try apply SRCC.
+    erewrite e2a_co; eauto.
+    rewrite !irreflexive_union. splits.
+    { apply hb_irr; eauto. }
+    { admit. }
+    (* { erewrite e2a_rf, e2a_jf; eauto. *)
+    (*   intros x [y [HB VF]]. *)
+    (*   unfold furr in VF. desc.   *)
+    (*   eapply urr_hb_irr; try apply SRCC. *)
+    (*   basic_solver. } *)
+    { arewrite (Gco ⊆ Geco^?).
+      2: by apply GCOH.
+      rewrite Execution_eco.co_in_eco. basic_solver. }
+    erewrite e2a_rf, e2a_jf; eauto.
+    intros x [y [HB [z [CO VF]]]].
+    unfold furr in VF. desc.  
+    eapply eco_urr_irr; try apply SRCC.
+    eexists. splits.
+    { unfold Execution_eco.eco. basic_solver 10. }
+    eapply urr_hb. basic_solver.
+  Admitted.
+
+  Lemma simrel_cert_step_consistent k k' e e' S S'
+        (st st' st'': (thread_st (ktid S k)))
+        (SRCC : simrel_cert prog S G sc TC TC' X k st st'')
+        (CertSTEP : cert_step G sc TC TC' X k k' st st' e e' S S')
+        (CST_REACHABLE : (lbl_step (ktid S k))＊ st' st'') : 
+    @es_consistent S' Weakestmo. 
+  Proof. 
+    cdes CertSTEP; cdes BSTEP_.
+    assert (basic_step e e' S S') as BSTEP.
+    { econstructor; eauto. }
+    assert (ES.Wf S) as WFS.
+    { apply SRCC. }
+    constructor.
+    { eapply ecf_irr_alt. split.
+      { eapply simrel_cert_step_hb_cf_irr; eauto. }
+      eapply simrel_cert_step_thb_cf_hb_irr; eauto. }
+    { eapply simrel_cert_step_jf_necf; eauto. }
+    { eapply simrel_cert_step_jfe_vis; eauto. }
+    { eapply simrel_cert_step_coh; eauto. }
+    { admit. }
+    admit. 
+  Admitted.
+
+  Lemma simrel_cert_lbl_step k S
+        (st st' st'': (thread_lts (ktid S k)).(Language.state))
+        (SRCC : simrel_cert prog S G sc TC TC' X k st st'')
+        (LBL_STEP : lbl_step (ktid S k) st st')
+        (CST_REACHABLE : (lbl_step (ktid S k))＊ st' st'') :
+    exists k' S',
+      ⟪ kTID : ktid S' k' = ktid S k ⟫ /\
+      ⟪ ESSTEP : (step Weakestmo)^? S S' ⟫ /\
+      ⟪ SRCC' : simrel_cert prog S' G sc TC TC' X k' st' st''⟫.
+  Proof.
+    edestruct LBL_STEP as [lbl ILBL_STEP].
+    edestruct simrel_cert_step as [k' HH]; eauto. desc.
+    cdes CertSTEP.
+    assert (ES.Wf S) as WFS.
+    { apply SRCC. }
+    assert (basic_step e e' S S') as BSTEP.
+    { econstructor; eauto. }
+    assert (step_ e e' S S') as WMO_STEP_.
+    { eapply simrel_cert_step_step_; eauto. }
+    exists k', S'. splits.
+    { eapply basic_step_cont_thread_k; eauto. }
+    { apply r_step. red.
+      do 2 eexists; splits; eauto.
+      eapply simrel_cert_step_consistent; eauto. }
+    constructor.
+    { red. splits.
+      { eapply simrel_cert_step_simrel_; eauto. }
+      eapply simrel_cert_step_consistent; eauto. }
+    (* tr_step : isim_trav_step G sc (ktid S k') TC TC' *)
+    { erewrite basic_step_cont_thread_k; eauto. apply SRCC. }
+    (* cert : cert_graph G sc TC TC' (ktid S k') state'' *)
+    { erewrite basic_step_cont_thread_k; eauto. apply SRCC. }
+    (* cstate : simrel_cstate *)
+    { eapply simrel_cert_basic_step_cstate; eauto. } 
+    all : admit.
+  Admitted.
+
+End SimRelCertStepCoh.
